PlusFold.v
@@ -22,17 +22,15 @@ s ==~ plus_fold (l1 ++ l2) <-> s ==~ (plus_fold l1) _+_ (plus_fold l2).
 Proof.
 intro. induction l1.
 - intros. split.
-  * intros. simpl in H. apply MPlusR. assumption.
+  * intros. simpl in H. auto.
   * intros. simpl. simpl in H. inversion H. {  inversion H2. } assumption.
 - intros. split.
-  * intros. simpl in *. apply plus_or in H as [H | H]. { apply MPlusL. apply MPlusL. assumption. }
-                                                       { specialize IHl1 with l2. apply IHl1 in H. 
-                                                         apply plus_assoc. apply MPlusR. assumption. } 
+  * intros. simpl in *. apply plus_or in H as [H | H] ; auto.
+    specialize IHl1 with l2. apply IHl1 in H. apply plus_assoc. auto.
   * intros. simpl in *. apply plus_assoc in H. apply plus_or in H as [H | H].
-    ** apply MPlusL. assumption.
+    ** auto.
     ** apply MPlusR. apply IHl1. assumption.
 Qed.
-
 
 
 Lemma in_plus_fold : forall (s : Trace)(l : list Contract), s ==~ plus_fold l <-> 
@@ -40,13 +38,36 @@ Lemma in_plus_fold : forall (s : Trace)(l : list Contract), s ==~ plus_fold l <-
 Proof.
 intros. split.
 - induction l.
-  * intros.  simpl in H. inversion H.
+  * intros. simpl in H. inversion H.
   * intros. simpl in H. apply plus_or in H as [H | H].
     ** exists a. split. apply in_eq. assumption.
-    ** apply IHl in H as [c' [P1 P2]]. exists c'. split. { apply in_cons. assumption. } { assumption. }
+    ** apply IHl in H as [c' [P1 P2]]. exists c'. split ; auto using  in_cons.
 - intros. destruct H as [ c' [P1 P2]]. induction l.
   * destruct P1.
   * apply in_inv in P1 as [P1 | P1].
-    ** simpl. rewrite P1. apply MPlusL. assumption. 
-    ** simpl.  apply MPlusR. auto.
+    ** simpl. rewrite P1. auto.
+    ** simpl. auto.
+Qed.
+
+
+
+plus_fold (map (fun s : Trace => seq_fold (map Event s)) (monoms c1 ++ monoms c2)) =R=
+c1 _+_ c2
+
+
+
+
+Fixpoint seq_fold (l : list Contract) :=
+match l with
+| [] => Success
+| a::l' => a _;_ (seq_fold l')
+end.
+
+
+
+Lemma seq_fold_map : forall (s:Trace), s ==~ seq_fold (map Event s).
+Proof.
+induction s.
+- simpl. auto.
+- simpl. assert (HA: a::s = [a]++s). { reflexivity. } rewrite HA. constructor; auto.
 Qed.
