Order.v
@@ -1,0 +1,100 @@
+Require Import CSL.Contract.
+Require Import Lists.List.
+Require Import Sorting.Permutation.
+Require Import Sorting.Mergesort.
+Require Import Sorting.Sorted.
+Require Import Bool.Bool.
+Require Import Bool.Sumbool.
+Require Import List Setoid Permutation Sorted Orders.
+Import ListNotations.
+
+Set Implicit Arguments.
+
+
+Module TraceOrder <: TotalLeBool.
+  Definition t := Trace.
+
+  (*Notify <= Transfer*)
+  Definition leb_event x y :=
+    match x, y with
+    | Transfer,Notify  => false
+    | _, _ => true
+    end.
+  (*leb_event is total, anti symmetric and transitive*)
+
+  Lemma leb_event_total : forall e1 e2, leb_event e1 e2 = true \/ leb_event e2 e1  = true.
+  Proof. intros. destruct e1 ; destruct e2 ; auto || auto. Defined.
+
+  Lemma leb_event_anti_sym : forall (e1 e2 : EventType), leb_event e1 e2 = leb_event e2 e1  ->  e1 = e2.
+  Proof.
+  intros. destruct e1 ; destruct e2 ; try reflexivity ; simpl in H ; simpl in H ; discriminate.
+  Qed. 
+
+(*  Lemma leb_event_anti_sym : forall (e1 e2 : EventType), TraceOrder.leb_event e1 e2 = true -> 
+  TraceOrder.leb_event e2 e1 = true -> e1 = e2.
+  Proof.
+  intros. destruct e1 ; destruct e2 ; try reflexivity ; simpl in H ; simpl in H0 ; discriminate.
+  Qed. *)
+
+  Lemma leb_event_trans : forall (x y z : EventType), leb_event x y = true -> leb_event y z = true -> leb_event x z = true.
+  Proof. intros. destruct x ; destruct y ; destruct z ; simpl in H ; simpl in H0 ; try reflexivity. 
+  - destruct H0. simpl. reflexivity.
+  - discriminate H.
+  Qed.
+
+
+  (*Lexicographic ordering of traces*)
+  Fixpoint leb s1 s2 :=
+    match s1, s2 with
+    | [],_ => true
+    | _,[] => false
+    | a1::s1',a2::s2' => if (eq_event_dec a1 a2) 
+                           then leb s1' s2' 
+                           else leb_event a1 a2
+    end.
+  Infix "<=?" := leb (at level 70, no associativity).
+
+  Lemma leb_anti_sym : forall s1 s2: Trace, s1 <=? s2 = (s2 <=? s1) -> s1 = s2.
+  Proof.
+  induction s1.
+  - intros. destruct s2 ; try reflexivity. simpl in H. discriminate.
+  - intros. destruct s2; simpl in H; try discriminate.
+    destruct (eq_event_dec a e).
+    ** rewrite e0. f_equal. destruct (eq_event_dec e a).
+      *** auto.
+      *** symmetry in e0. contradiction.
+    ** destruct (eq_event_dec e a) ; try (symmetry in e0 ; contradiction).
+       apply leb_event_anti_sym in H. contradiction.
+  Qed.
+
+  Lemma leb_trans : Transitive (fun s1 s2 => leb s1 s2 = true).
+  Proof. unfold Transitive. induction x.
+  - intros. reflexivity.
+  - intros. destruct y ; destruct z ; try reflexivity ; try (simpl in H ; discriminate).
+    simpl. destruct (eq_event_dec a e0). 
+    * simpl in H. destruct (eq_event_dec a e).
+      ** simpl in H0. subst. destruct (eq_event_dec e0 e0) ; try contradiction.
+         eauto.
+      ** simpl in H0. subst. destruct (eq_event_dec e e0).
+        *** subst. contradiction.
+        *** rewrite <- H0 in H. apply leb_event_anti_sym in H. contradiction.
+    * simpl in H. destruct (eq_event_dec a e).
+      ** simpl in H0. subst. destruct (eq_event_dec e e0) ; [ contradiction | assumption ].
+      ** simpl in H0. destruct (eq_event_dec e e0).
+        *** subst. assumption.
+        *** eauto using leb_event_trans.
+  Qed.
+
+
+  Theorem leb_total : forall a1 a2, a1 <=? a2 = true \/ a2 <=? a1 = true.
+  Proof.
+  induction a1.
+    - intros. simpl. now left.
+    - destruct a2.
+      * simpl. now right.
+      * simpl. destruct (eq_event_dec a e) ; destruct (eq_event_dec e a) ;
+               destruct (IHa1 a2) ; auto using leb_event_total || auto using leb_event_total.
+  Defined.
+
+  Definition leb_prop s1 s2 := s1 <=? s2 = true.
+End TraceOrder.
